src/Core/Domain/Split_State.thy
@@ -22,6 +22,124 @@ text \<open>
 
 type_synonym ('l, 'g) split_state = "'l abs_state \<times> 'g abs_state"
 
+
+subsection \<open>Placement interface\<close>
+
+text \<open>
+  Placement controls which abstract component constrains a location.  It is
+  independent of source storage: a location can be constrained by the local
+  component, the side component, both components, or neither component.
+\<close>
+
+locale state_placement =
+  fixes keep_local :: "'loc => bool"
+    and publish_side :: "'loc => bool"
+begin
+
+definition placement_complete :: bool where
+  "placement_complete \<longleftrightarrow>
+    (\<forall>loc. keep_local loc \<or> publish_side loc)"
+
+definition placement_disjoint :: bool where
+  "placement_disjoint \<longleftrightarrow>
+    (\<forall>loc. \<not> (keep_local loc \<and> publish_side loc))"
+
+definition wf_components ::
+    "('loc => 'l::bot) => ('loc => 'g::bot) => bool" where
+  "wf_components local side \<longleftrightarrow>
+    (\<forall>loc. \<not> keep_local loc \<longrightarrow> local loc = bot) \<and>
+    (\<forall>loc. \<not> publish_side loc \<longrightarrow> side loc = bot)"
+
+definition gamma_components ::
+    "('loc => 'l::sound_domain) => ('loc => 'g::sound_domain)
+      => ('loc => int) set" where
+  "gamma_components local side =
+    {s. \<forall>loc.
+      (keep_local loc \<longrightarrow> s loc \<in> gamma (local loc)) \<and>
+      (publish_side loc \<longrightarrow> s loc \<in> gamma (side loc))}"
+
+lemma gamma_componentsD_local [dest]:
+  assumes "s \<in> gamma_components local side" and "keep_local loc"
+  shows "s loc \<in> gamma (local loc)"
+  using assms unfolding gamma_components_def by blast
+
+lemma gamma_componentsD_side [dest]:
+  assumes "s \<in> gamma_components local side" and "publish_side loc"
+  shows "s loc \<in> gamma (side loc)"
+  using assms unfolding gamma_components_def by blast
+
+
+lemma gamma_componentsD_covered:
+  assumes complete: placement_complete
+    and member: "s \<in> gamma_components local side"
+  shows "s loc \<in> gamma (local loc) \<or> s loc \<in> gamma (side loc)"
+  using complete member
+  unfolding placement_complete_def gamma_components_def by blast
+lemma gamma_components_update_unconstrained:
+  assumes "s \<in> gamma_components local side"
+    and "\<not> keep_local loc"
+    and "\<not> publish_side loc"
+  shows "s(loc := value) \<in> gamma_components local side"
+  using assms unfolding gamma_components_def by auto
+
+end
+
+
+context state_placement
+begin
+
+lemma wf_components_bot:
+  "wf_components (bot :: 'loc => 'l::bot) (bot :: 'loc => 'g::bot)"
+  unfolding wf_components_def bot_fun_def by simp
+
+lemma wf_components_sup:
+  fixes local1 local2 :: "'loc => 'l::bounded_semilattice_sup_bot"
+    and side1 side2 :: "'loc => 'g::bounded_semilattice_sup_bot"
+  assumes "wf_components local1 side1" and "wf_components local2 side2"
+  shows "wf_components (local1 \<squnion> local2) (side1 \<squnion> side2)"
+  using assms unfolding wf_components_def by (simp add: sup_fun_def)
+
+end
+
+definition project_component ::
+  "('loc => bool) => ('loc => 'a::bot) => 'loc => 'a" where
+  "project_component placed state =
+     (\<lambda>loc. if placed loc then state loc else bot)"
+
+definition sequential_keep_local :: "'loc => bool" where
+  "sequential_keep_local loc = True"
+
+definition sequential_publish_side :: "'loc => bool" where
+  "sequential_publish_side loc = False"
+
+definition classic_keep_local :: "(vname => bool) => vname => bool" where
+  "classic_keep_local storage loc = (\<not> storage loc)"
+
+definition classic_publish_side :: "(vname => bool) => vname => bool" where
+  "classic_publish_side storage loc = storage loc"
+
+
+
+lemma sequential_placement_complete [simp]:
+  "state_placement.placement_complete
+    sequential_keep_local sequential_publish_side"
+  unfolding state_placement.placement_complete_def
+    sequential_keep_local_def sequential_publish_side_def by simp
+
+lemma classic_placement_complete [simp]:
+  "state_placement.placement_complete
+    (classic_keep_local storage) (classic_publish_side storage)"
+  unfolding state_placement.placement_complete_def
+    classic_keep_local_def classic_publish_side_def by simp
+
+lemma classic_placement_disjoint [simp]:
+  "state_placement.placement_disjoint
+    (classic_keep_local storage) (classic_publish_side storage)"
+  unfolding state_placement.placement_disjoint_def
+    classic_keep_local_def classic_publish_side_def by simp
+
+
+
 subsection \<open>Well-formedness\<close>
 
 definition wf_split :: "('l::bot, 'g::bot) split_state \<Rightarrow> bool" where
@@ -69,6 +187,14 @@ definition split_state_for ::
   "split_state_for gs \<sigma> =
      ((%x. if gs x then bot else \<sigma> x),
       (%x. if gs x then \<sigma> x else bot))"
+
+lemma wf_components_classic_iff:
+  "state_placement.wf_components
+      (classic_keep_local storage) (classic_publish_side storage)
+      (fst split) (snd split)
+    \<longleftrightarrow> wf_split_for storage split"
+  unfolding state_placement.wf_components_def classic_keep_local_def
+    classic_publish_side_def wf_split_for_def by simp
 
 lemma merge_split_for [simp]:
   "merge_state_for gs (split_state_for gs \<sigma>) = \<sigma>"
