src/Core/Domain/Exec_Placement.thy
@@ -1,0 +1,443 @@
+theory Exec_Placement
+  imports Exec_St "Voblint_VIMP.VIMP_Notation"
+begin
+
+section \<open>Finite executable placement scopes\<close>
+
+type_synonym scoped_location = "pname * location"
+
+definition scoped_location_of :: "pname => location => scoped_location" where
+  "scoped_location_of owner loc = (owner, loc)"
+
+definition placement_global_invariant ::
+  "(scoped_location => bool) => bool" where
+  "placement_global_invariant placed \<longleftrightarrow>
+    (\<forall>p q x. placed (p, Global_Location x) = placed (q, Global_Location x))"
+
+definition classic_keep_local :: "scoped_location => bool" where
+  "classic_keep_local scoped =
+    (case snd scoped of Local_Location _ => True | Global_Location _ => False)"
+
+definition classic_publish_side :: "scoped_location => bool" where
+  "classic_publish_side scoped =
+    (case snd scoped of Local_Location _ => False | Global_Location _ => True)"
+
+lemma classic_keep_local_global_invariant:
+  "placement_global_invariant classic_keep_local"
+  unfolding placement_global_invariant_def classic_keep_local_def by simp
+
+lemma classic_publish_side_global_invariant:
+  "placement_global_invariant classic_publish_side"
+  unfolding placement_global_invariant_def classic_publish_side_def by simp
+
+definition scope_locations :: "imp_prog => pname => location list" where
+  "scope_locations p owner =
+    remdups (map (location_of (storage_global p owner))
+      (scope_vnames_list p owner))"
+
+lemma set_scope_locations [simp]:
+  "set (scope_locations p owner) =
+    image (location_of (storage_global p owner)) (scope_vnames p owner)"
+  unfolding scope_locations_def
+  by simp
+
+lemma declared_global_in_scope_locations:
+  assumes "declared_global p x"
+  shows "Global_Location x \<in> set (scope_locations p owner)"
+proof -
+  have x_scope: "x \<in> scope_vnames p owner"
+    using assms unfolding scope_vnames_def by simp
+  have location:
+    "location_of (storage_global p owner) x = Global_Location x"
+    using assms by (simp add: location_of_def)
+  have member:
+    "location_of (storage_global p owner) x \<in>
+      image (location_of (storage_global p owner)) (scope_vnames p owner)"
+    by (rule imageI[OF x_scope])
+  show ?thesis
+    using member location by simp
+qed
+
+lemma implicit_local_in_scope_locations:
+  assumes "x \<in> scope_vnames p owner" and "\<not> declared_global p x"
+  shows "Local_Location x \<in> set (scope_locations p owner)"
+proof -
+  have location:
+    "location_of (storage_global p owner) x = Local_Location x"
+    using assms by (simp add: location_of_def)
+  have member:
+    "location_of (storage_global p owner) x \<in>
+      image (location_of (storage_global p owner)) (scope_vnames p owner)"
+    by (rule imageI[OF assms(1)])
+  show ?thesis
+    using member location by simp
+qed
+
+subsection \<open>Materialized placement projection\<close>
+
+fun resolved_default :: "('a::bot) resolved_st => location => 'a" where
+  "resolved_default (dl, dg, entries) (Local_Location x) = dl"
+| "resolved_default (dl, dg, entries) (Global_Location x) = dg"
+
+fun raw_support :: "('a::bot) resolved_st => location list" where
+  "raw_support (dl, dg, entries) = map fst entries"
+
+definition effective_support ::
+  "('a::bot) resolved_st => location list" where
+  "effective_support s =
+    filter (\<lambda>loc. lookup_resolved_st s loc \<noteq> resolved_default s loc)
+      (remdups (raw_support s))"
+
+definition relevant_locations ::
+  "imp_prog => pname => ('a::bot) resolved_st => location list" where
+  "relevant_locations p owner s =
+    remdups (scope_locations p owner @ effective_support s)"
+
+lemma set_relevant_locations [simp]:
+  "set (relevant_locations p owner s) =
+    set (scope_locations p owner) \<union> set (effective_support s)"
+  unfolding relevant_locations_def by simp
+
+lemma set_effective_support:
+  "set (effective_support s) =
+    {loc \<in> set (raw_support s).
+      lookup_resolved_st s loc \<noteq> resolved_default s loc}"
+  unfolding effective_support_def
+  by auto
+
+lemma eq_resolved_st_defaults:
+  assumes "eq_resolved_st (dl, dg, ps) (el, eg, qs)"
+  shows "dl = el \<and> dg = eg"
+proof -
+  obtain x where fresh:
+    "x \<notin> image location_vname (set (map fst ps @ map fst qs))"
+    using fresh_vname_notin[of ps qs] by auto
+  have local_support:
+    "Local_Location x \<notin> set (map fst ps @ map fst qs)"
+  proof
+    assume "Local_Location x \<in> set (map fst ps @ map fst qs)"
+    then have "location_vname (Local_Location x) \<in>
+        image location_vname (set (map fst ps @ map fst qs))"
+      by (rule imageI)
+    with fresh show False by simp
+  qed
+  have global_support:
+    "Global_Location x \<notin> set (map fst ps @ map fst qs)"
+  proof
+    assume "Global_Location x \<in> set (map fst ps @ map fst qs)"
+    then have "location_vname (Global_Location x) \<in>
+        image location_vname (set (map fst ps @ map fst qs))"
+      by (rule imageI)
+    with fresh show False by simp
+  qed
+  have local_ps: "map_of ps (Local_Location x) = None"
+    using local_support by (simp add: map_of_resolved_none_iff)
+  have local_qs: "map_of qs (Local_Location x) = None"
+    using local_support by (simp add: map_of_resolved_none_iff)
+  have global_ps: "map_of ps (Global_Location x) = None"
+    using global_support by (simp add: map_of_resolved_none_iff)
+  have global_qs: "map_of qs (Global_Location x) = None"
+    using global_support by (simp add: map_of_resolved_none_iff)
+  have lookup:
+    "lookup_resolved_st (dl, dg, ps) =
+      lookup_resolved_st (el, eg, qs)"
+    using assms unfolding eq_resolved_st_def by simp
+  have local_lookup:
+    "lookup_resolved_st (dl, dg, ps) (Local_Location x) =
+      lookup_resolved_st (el, eg, qs) (Local_Location x)"
+    using lookup by (rule fun_cong)
+  have local_eq: "dl = el"
+    using local_ps local_qs local_lookup by simp
+  have global_lookup:
+    "lookup_resolved_st (dl, dg, ps) (Global_Location x) =
+      lookup_resolved_st (el, eg, qs) (Global_Location x)"
+    using lookup by (rule fun_cong)
+  have global_eq: "dg = eg"
+    using global_ps global_qs global_lookup by simp
+  show ?thesis using local_eq global_eq by simp
+qed
+
+lemma lookup_resolved_st_eq_default:
+  assumes "loc \<notin> set (raw_support s)"
+  shows "lookup_resolved_st s loc = resolved_default s loc"
+proof (cases s)
+  case (fields dl dg entries)
+  have entries_none: "map_of entries loc = None"
+    using assms fields
+    by (simp add: raw_support.simps map_of_resolved_none_iff)
+  show ?thesis
+    using fields entries_none by (cases loc) simp_all
+qed
+
+lemma effective_support_mem_eq:
+  assumes eq: "eq_resolved_st (dl, dg, ps) (el, eg, qs)"
+    and loc: "loc \<in> set (effective_support (dl, dg, ps))"
+  shows "loc \<in> set (effective_support (el, eg, qs))"
+proof -
+  have loc_ps: "loc \<in> set (map fst ps)"
+    and unequal: "lookup_resolved_st (dl, dg, ps) loc \<noteq>
+      resolved_default (dl, dg, ps) loc"
+    using loc by (auto simp: set_effective_support raw_support.simps)
+  have defaults: "dl = el \<and> dg = eg"
+    using eq by (rule eq_resolved_st_defaults)
+  have lookup:
+    "lookup_resolved_st (dl, dg, ps) =
+      lookup_resolved_st (el, eg, qs)"
+    using eq unfolding eq_resolved_st_def by simp
+  have lookup_loc:
+    "lookup_resolved_st (dl, dg, ps) loc =
+      lookup_resolved_st (el, eg, qs) loc"
+    using lookup by (rule fun_cong)
+  have loc_qs: "loc \<in> set (map fst qs)"
+  proof (rule ccontr)
+    assume not_qs: "\<not> loc \<in> set (map fst qs)"
+    have qs_not: "loc \<notin> set (raw_support (el, eg, qs))"
+      using not_qs by simp
+    have qs_value:
+      "lookup_resolved_st (el, eg, qs) loc =
+        resolved_default (el, eg, qs) loc"
+      using qs_not by (rule lookup_resolved_st_eq_default)
+    show False
+      using unequal defaults qs_value lookup_loc
+      by (cases loc) simp_all
+  qed
+  have target_unequal:
+    "lookup_resolved_st (el, eg, qs) loc \<noteq>
+      resolved_default (el, eg, qs) loc"
+  proof
+    assume target_eq:
+      "lookup_resolved_st (el, eg, qs) loc =
+        resolved_default (el, eg, qs) loc"
+    show False
+      using unequal defaults target_eq lookup_loc
+      by (cases loc) simp_all
+  qed
+  show ?thesis
+    using loc_qs target_unequal
+    by (auto simp: set_effective_support raw_support.simps)
+qed
+
+lemma eq_resolved_st_effective_support:
+  assumes "eq_resolved_st (dl, dg, ps) (el, eg, qs)"
+  shows
+    "set (effective_support (dl, dg, ps)) =
+      set (effective_support (el, eg, qs))"
+proof (rule subset_antisym)
+  show "set (effective_support (dl, dg, ps)) \<subseteq>
+      set (effective_support (el, eg, qs))"
+    using assms by (auto intro: effective_support_mem_eq)
+next
+  show "set (effective_support (el, eg, qs)) \<subseteq>
+      set (effective_support (dl, dg, ps))"
+    using assms
+    by (auto intro: effective_support_mem_eq[OF
+      equivp_symp[OF equivp_eq_resolved_st]])
+qed
+
+
+definition project_resolved_on_raw ::
+  "pname => location list => (scoped_location => bool) =>
+   ('a::bot) resolved_st => 'a resolved_st" where
+  "project_resolved_on_raw owner universe placed s =
+    foldr (\<lambda>loc result.
+      if placed (owner, loc)
+      then update_resolved_st result loc (lookup_resolved_st s loc)
+      else result)
+    (remdups (universe @ effective_support s)) (bot, bot, [])"
+lemma lookup_materialize_locations:
+  fixes locations :: "location list"
+  shows
+    "lookup_resolved_st
+      (foldr (\<lambda>loc result.
+        if placed (owner, loc)
+        then update_resolved_st result loc (lookup_resolved_st s loc)
+        else result)
+        locations (bot, bot, [])) target =
+      (if target \<in> set locations \<and> placed (owner, target)
+       then lookup_resolved_st s target else bot)"
+proof (induction locations)
+  case Nil
+  then show ?case by (cases target) simp_all
+next
+  case (Cons loc locations)
+  show ?case
+  proof (cases "loc = target")
+    case True
+    show ?thesis
+    proof (cases "placed (owner, target)")
+      case True
+      with `loc = target` show ?thesis by simp
+    next
+      case False
+      with `loc = target` Cons.IH show ?thesis by simp
+    qed
+  next
+    case False
+    then show ?thesis
+      using Cons by (simp add: lookup_resolved_st_update_diff)
+  qed
+qed
+
+lemma lookup_project_resolved_on_raw:
+  "lookup_resolved_st (project_resolved_on_raw owner universe placed s) target =
+    (if target \<in> set (remdups (universe @ effective_support s)) \<and>
+        placed (owner, target)
+     then lookup_resolved_st s target else bot)"
+  unfolding project_resolved_on_raw_def
+  by (rule lookup_materialize_locations)
+
+lemma lookup_project_resolved_on_raw_relevant:
+  assumes "target \<in> set (universe @ effective_support s)"
+  shows
+    "lookup_resolved_st (project_resolved_on_raw owner universe placed s) target =
+      (if placed (owner, target) then lookup_resolved_st s target else bot)"
+  using assms by (simp add: lookup_project_resolved_on_raw)
+
+lemma eq_resolved_st_project_resolved_on_raw:
+  assumes eq: "eq_resolved_st s t"
+  shows "eq_resolved_st
+    (project_resolved_on_raw owner universe placed s)
+    (project_resolved_on_raw owner universe placed t)"
+proof -
+  obtain dl dg ps where s: "s = (dl, dg, ps)"
+    by (cases s)
+  obtain el eg qs where t: "t = (el, eg, qs)"
+    by (cases t)
+  have effective:
+    "set (effective_support s) = set (effective_support t)"
+    using eq s t by (simp add: eq_resolved_st_effective_support)
+  have lookup: "lookup_resolved_st s = lookup_resolved_st t"
+    using eq unfolding eq_resolved_st_def by simp
+  show ?thesis
+    unfolding eq_resolved_st_def
+  proof (rule ext)
+    fix target
+    have relevant:
+      "target \<in> set (remdups (universe @ effective_support s)) \<longleftrightarrow>
+        target \<in> set (remdups (universe @ effective_support t))"
+      using effective by simp
+    show "lookup_resolved_st
+      (project_resolved_on_raw owner universe placed s) target =
+      lookup_resolved_st
+      (project_resolved_on_raw owner universe placed t) target"
+      using relevant lookup
+      by (simp add: lookup_project_resolved_on_raw fun_eq_iff)
+  qed
+qed
+
+lift_definition project_resolved_on ::
+  "pname => location list => (scoped_location => bool) =>
+   ('a::bot) resolved_st_q => 'a resolved_st_q"
+  is project_resolved_on_raw
+  by (rule eq_resolved_st_project_resolved_on_raw)
+
+lemma project_resolved_on_Abs:
+  "project_resolved_on owner universe placed (Abs_resolved_st s) =
+    Abs_resolved_st (project_resolved_on_raw owner universe placed s)"
+  by transfer (simp add: eq_resolved_st_def)
+
+lemma lookup_project_resolved_on_Abs:
+  "lookup_resolved_st_q
+    (project_resolved_on owner universe placed (Abs_resolved_st s)) target =
+    (if target \<in> set (remdups (universe @ effective_support s)) \<and>
+        placed (owner, target)
+     then lookup_resolved_st s target else bot)"
+  by (simp add: project_resolved_on_Abs lookup_project_resolved_on_raw)
+
+lemma lookup_project_resolved_on:
+  "lookup_resolved_st_q
+    (project_resolved_on owner universe placed s) target =
+    (if target \<in>
+        set (remdups
+          (universe @ effective_support (rep_resolved_st s))) \<and>
+        placed (owner, target)
+     then lookup_resolved_st_q s target else bot)"
+proof -
+  have abs: "Abs_resolved_st (rep_resolved_st s) = s"
+    by simp
+  show ?thesis
+    using lookup_project_resolved_on_Abs[
+      of owner universe placed "rep_resolved_st s" target]
+    unfolding abs
+    by (simp add: lookup_rep_resolved_st_q)
+qed
+
+lemma lookup_project_resolved_on_relevant:
+  assumes "target \<in>
+    set (universe @ effective_support (rep_resolved_st s))"
+  shows
+    "lookup_resolved_st_q
+      (project_resolved_on owner universe placed s) target =
+      (if placed (owner, target)
+       then lookup_resolved_st_q s target else bot)"
+  using assms by (simp add: lookup_project_resolved_on)
+
+
+lemma lookup_project_resolved_on_join:
+  fixes s :: "('a::bounded_semilattice_sup_bot) resolved_st_q"
+  assumes relevant:
+    "target \<in> set (universe @ effective_support (rep_resolved_st s))"
+    and covered: "keep_local (owner, target) \<or> publish_side (owner, target)"
+  shows
+    "lookup_resolved_st_q
+      (project_resolved_on owner universe keep_local s \<squnion>
+       project_resolved_on owner universe publish_side s) target =
+      lookup_resolved_st_q s target"
+proof (cases "keep_local (owner, target)")
+  case True
+  with relevant show ?thesis
+    by (simp add: lookup_project_resolved_on_relevant)
+next
+  case False
+  with covered have publish: "publish_side (owner, target)"
+    by simp
+  with relevant show ?thesis
+    by (simp add: lookup_project_resolved_on_relevant)
+qed
+
+lemma lookup_project_resolved_on_classic_local:
+  fixes s :: "('a::bounded_semilattice_sup_bot) resolved_st_q"
+  assumes relevant:
+    "target \<in> set (universe @ effective_support (rep_resolved_st s))"
+  shows
+    "lookup_resolved_st_q
+      (project_resolved_on owner universe classic_keep_local s) target =
+      lookup_resolved_st_q (restrict_local_resolved_q s) target"
+proof (cases target)
+  case (Local_Location x)
+  then show ?thesis
+    using relevant
+    by (simp add: classic_keep_local_def
+      lookup_project_resolved_on_relevant)
+next
+  case (Global_Location x)
+  then show ?thesis
+    using relevant
+    by (simp add: classic_keep_local_def
+      lookup_project_resolved_on_relevant)
+qed
+
+lemma lookup_project_resolved_on_classic_side:
+  fixes s :: "('a::bounded_semilattice_sup_bot) resolved_st_q"
+  assumes relevant:
+    "target \<in> set (universe @ effective_support (rep_resolved_st s))"
+  shows
+    "lookup_resolved_st_q
+      (project_resolved_on owner universe classic_publish_side s) target =
+      lookup_resolved_st_q (restrict_global_resolved_q s) target"
+proof (cases target)
+  case (Local_Location x)
+  then show ?thesis
+    using relevant
+    by (simp add: classic_publish_side_def
+      lookup_project_resolved_on_relevant)
+next
+  case (Global_Location x)
+  then show ?thesis
+    using relevant
+    by (simp add: classic_publish_side_def
+      lookup_project_resolved_on_relevant)
+qed
+
+end
+
