src/Examples/Interval/Example_Interval_Placement.thy
@@ -1,0 +1,136 @@
+theory Example_Interval_Placement
+  imports "Voblint_Analysis.Ivl_Exec"
+begin
+
+hide_const phase.N
+
+section \<open>Interval placement slice with independent global policies\<close>
+
+text \<open>
+  The program has two declared globals with independent placement.  The procedure
+  call binds a formal, introduces the implicit local \<open>tmp\<close>, and returns into the
+  caller-local \<open>answer\<close>.  Neither global name relies on the historical \<open>G\<close>
+  prefix convention.
+\<close>
+
+definition placement_prog :: imp_prog where
+  "placement_prog = program {
+     global balance, request_count;
+     void add(x) {
+       tmp := balance + x;
+       balance := tmp;
+       request_count := request_count + 1;
+       return balance
+     }
+     void main() { answer := add(3) }
+   }"
+
+definition placement_owner :: pname where
+  "placement_owner = ''add''"
+
+fun placement_keep_local :: "scoped_location => bool" where
+  "placement_keep_local (owner, Local_Location x) = True"
+| "placement_keep_local (owner, Global_Location x) = (x = ''balance'')"
+
+fun placement_publish_side :: "scoped_location => bool" where
+  "placement_publish_side (owner, Local_Location x) = False"
+| "placement_publish_side (owner, Global_Location x) = (x = ''request_count'')"
+
+lemma placement_keep_local_global_invariant:
+  "placement_global_invariant placement_keep_local"
+  unfolding placement_global_invariant_def by simp
+
+lemma placement_publish_side_global_invariant:
+  "placement_global_invariant placement_publish_side"
+  unfolding placement_global_invariant_def by simp
+
+definition placement_state :: "ivl resolved_st_q" where
+  "placement_state =
+    update_resolved_st_q
+      (update_resolved_st_q cinit_ivl_st (Global_Location ''balance'')
+        (Ivl (Fin 10) (Fin 10)))
+      (Global_Location ''request_count'') (Ivl (Fin 4) (Fin 4))"
+
+definition placement_local_state :: "ivl resolved_st_q" where
+  "placement_local_state =
+    project_resolved_on placement_owner
+      (scope_locations placement_prog placement_owner)
+      placement_keep_local placement_state"
+
+definition placement_side_state :: "ivl resolved_st_q" where
+  "placement_side_state =
+    project_resolved_on placement_owner
+      (scope_locations placement_prog placement_owner)
+      placement_publish_side placement_state"
+
+subsection \<open>Source storage and finite call scope\<close>
+
+lemma placement_storage:
+  "storage_of placement_prog ''add'' ''balance'' = GlobalVar"
+  "storage_of placement_prog ''add'' ''request_count'' = GlobalVar"
+  "storage_of placement_prog ''add'' ''x'' = LocalVar ''add''"
+  "storage_of placement_prog ''add'' ''tmp'' = LocalVar ''add''"
+  "storage_of placement_prog prog_main_name ''answer'' = LocalVar prog_main_name"
+  by eval+
+
+lemma placement_add_scope:
+  "Global_Location ''balance'' \<in> set (scope_locations placement_prog placement_owner)"
+  "Global_Location ''request_count'' \<in> set (scope_locations placement_prog placement_owner)"
+  "Local_Location ''x'' \<in> set (scope_locations placement_prog placement_owner)"
+  "Local_Location ''tmp'' \<in> set (scope_locations placement_prog placement_owner)"
+  "Local_Location ret_var \<in> set (scope_locations placement_prog placement_owner)"
+  by eval+
+
+lemma placement_main_scope:
+  "Local_Location ''answer'' \<in>
+    set (scope_locations placement_prog prog_main_name)"
+  by eval
+
+subsection \<open>Selective executable projection\<close>
+
+lemma placement_local_projection:
+  "lookup_resolved_st_q placement_local_state (Global_Location ''balance'') =
+    Ivl (Fin 10) (Fin 10)"
+  "lookup_resolved_st_q placement_local_state (Global_Location ''request_count'') = bot"
+  "lookup_resolved_st_q placement_side_state (Global_Location ''balance'') = bot"
+  "lookup_resolved_st_q placement_side_state (Global_Location ''request_count'') =
+    Ivl (Fin 4) (Fin 4)"
+  by eval+
+
+lemma placement_local_formal:
+  "lookup_resolved_st_q placement_local_state (Local_Location ''x'') =
+    Ivl MinInf PlusInf"
+  "lookup_resolved_st_q placement_local_state (Local_Location ''tmp'') =
+    Ivl MinInf PlusInf"
+  by eval+
+
+lemma placement_join_recovers_globals:
+  "lookup_resolved_st_q
+    (placement_local_state \<squnion> placement_side_state)
+    (Global_Location ''balance'') =
+    lookup_resolved_st_q placement_state (Global_Location ''balance'')"
+  "lookup_resolved_st_q
+    (placement_local_state \<squnion> placement_side_state)
+    (Global_Location ''request_count'') =
+    lookup_resolved_st_q placement_state (Global_Location ''request_count'')"
+  by eval+
+
+lemma placement_classic_projection:
+  "lookup_resolved_st_q
+    (project_resolved_on placement_owner
+      (scope_locations placement_prog placement_owner)
+      Exec_Placement.classic_keep_local placement_state)
+    (Global_Location ''balance'') =
+    lookup_resolved_st_q (restrict_local_resolved_q placement_state)
+      (Global_Location ''balance'')"
+  "lookup_resolved_st_q
+    (project_resolved_on placement_owner
+      (scope_locations placement_prog placement_owner)
+      Exec_Placement.classic_publish_side placement_state)
+    (Global_Location ''request_count'') =
+    lookup_resolved_st_q (restrict_global_resolved_q placement_state)
+      (Global_Location ''request_count'')"
+  by eval+
+
+end
+
